vale/code/arch/x64/X64.Memory_s.fsti
@@ -466,7 +466,9 @@ val lemma_valid_taint64: (b:buffer64) ->
                          (i:nat{i < buffer_length b}) ->
                          (t:taint) -> Lemma
   (requires valid_taint_buf64 b mem memTaint t /\ buffer_readable mem b)
-  (ensures Map.sel memTaint (buffer_addr b mem + 8 `op_Multiply` i) == t)
+  (ensures (
+    let ptr = buffer_addr b mem + 8 `op_Multiply` i in
+    forall i'. i' >= ptr /\ i' < ptr + 8 ==> Map.sel memTaint i' == t))
 
 val lemma_valid_taint128: (b:buffer128) ->
                          (memTaint:memtaint) ->
@@ -474,7 +476,9 @@ val lemma_valid_taint128: (b:buffer128) ->
                          (i:nat{i < buffer_length b}) ->
                          (t:taint) -> Lemma
   (requires valid_taint_buf128 b mem memTaint t /\ buffer_readable mem b)
-  (ensures Map.sel memTaint (buffer_addr b mem + 16 `op_Multiply` i) == t /\ Map.sel memTaint (buffer_addr b mem + 16 `op_Multiply` i + 8) == t)
+  (ensures ( 
+    let ptr = buffer_addr b mem + 16 `op_Multiply` i in
+    forall i'. i' >= ptr /\ i' < ptr + 16 ==> Map.sel memTaint i' == t))
 
 val same_memTaint64: (b:buffer64) ->
                    (mem0:mem) ->
